src/Config.v
@@ -88,73 +88,73 @@ Section Config.
     - destruct x as [[] |], y as [[] |], z as [[] |]; simpl; intuition.
   Qed.
 
-  Definition monotonic_at (p : perm) (n : nat) (x y : config) : Prop :=
-    @guar _ specConfig p x y -> lifetime_lte (lifetime x n) (lifetime y n).
+  (* Definition monotonic_at (p : perm) (n : nat) (x y : config) : Prop := *)
+  (*   @guar _ specConfig p x y -> lifetime_lte (lifetime x n) (lifetime y n). *)
 
-  Instance monotonic_at_reflexive p n : Reflexive (monotonic_at p n).
-  Proof.
-    repeat intro. reflexivity.
-  Qed.
+  (* Instance monotonic_at_reflexive p n : Reflexive (monotonic_at p n). *)
+  (* Proof. *)
+  (*   repeat intro. reflexivity. *)
+  (* Qed. *)
 
-  Lemma bottom_monotonic_at n : forall x y, monotonic_at bottom_perm n x y.
-  Proof.
-    repeat intro. simpl in H. subst. reflexivity.
-  Qed.
+  (* Lemma bottom_monotonic_at n : forall x y, monotonic_at bottom_perm n x y. *)
+  (* Proof. *)
+  (*   repeat intro. simpl in H. subst. reflexivity. *)
+  (* Qed. *)
 
-  Definition monotonic (P : Perms) (n : nat) : Prop :=
-    forall p, p ∈ P -> exists p', p' <= p /\ p' ∈ P /\ forall x y, monotonic_at p' n x y.
+  (* Definition monotonic (P : Perms) (n : nat) : Prop := *)
+  (*   forall p, p ∈ P -> exists p', p' <= p /\ p' ∈ P /\ forall x y, monotonic_at p' n x y. *)
 
-  Lemma monotonic_bottom n : monotonic bottom_Perms n.
-  Proof.
-    repeat intro. exists bottom_perm. split; [| split].
-    apply bottom_perm_is_bottom. auto. apply bottom_monotonic_at.
-  Qed.
+  (* Lemma monotonic_bottom n : monotonic bottom_Perms n. *)
+  (* Proof. *)
+  (*   repeat intro. exists bottom_perm. split; [| split]. *)
+  (*   apply bottom_perm_is_bottom. auto. apply bottom_monotonic_at. *)
+  (* Qed. *)
 
-  Program Definition restrict_monotonic_at (p : perm) (n : nat) : perm :=
-    {|
-    pre := pre p;
-    rely := rely p;
-    guar := fun x y => guar p x y /\ monotonic_at p n x y;
-    |}.
-  Next Obligation.
-    constructor; repeat intro.
-    - split; intuition.
-    - destruct H, H0. split; [etransitivity; eauto |]. intro. etransitivity; eauto.
-  Qed.
-  Next Obligation.
-    respects.
-  Qed.
+  (* Program Definition restrict_monotonic_at (p : perm) (n : nat) : perm := *)
+  (*   {| *)
+  (*   pre := pre p; *)
+  (*   rely := rely p; *)
+  (*   guar := fun x y => guar p x y /\ monotonic_at p n x y; *)
+  (*   |}. *)
+  (* Next Obligation. *)
+  (*   constructor; repeat intro. *)
+  (*   - split; intuition. *)
+  (*   - destruct H, H0. split; [etransitivity; eauto |]. intro. etransitivity; eauto. *)
+  (* Qed. *)
+  (* Next Obligation. *)
+  (*   respects. *)
+  (* Qed. *)
 
-  Lemma restrict_monotonic_at_monotone p p' n :
-    p <= p' -> restrict_monotonic_at p n <= restrict_monotonic_at p' n.
-  Proof.
-    intros []. constructor; intros; simpl; auto. destruct H.
-    split; auto. intro. auto.
-  Qed.
+  (* Lemma restrict_monotonic_at_monotone p p' n : *)
+  (*   p <= p' -> restrict_monotonic_at p n <= restrict_monotonic_at p' n. *)
+  (* Proof. *)
+  (*   intros []. constructor; intros; simpl; auto. destruct H. *)
+  (*   split; auto. intro. auto. *)
+  (* Qed. *)
 
-  Lemma restrict_monotonic_at_lte p n : restrict_monotonic_at p n <= p.
-  Proof.
-    constructor; intros; simpl in *; intuition.
-  Qed.
+  (* Lemma restrict_monotonic_at_lte p n : restrict_monotonic_at p n <= p. *)
+  (* Proof. *)
+  (*   constructor; intros; simpl in *; intuition. *)
+  (* Qed. *)
 
-  Definition invariant_at (p : @perm _ specConfig) (n : nat) : Prop :=
-    forall l1 l2 x y, guar p x y <-> guar p (replace_lifetime x n l1) (replace_lifetime y n l2).
+  (* Definition invariant_at (p : @perm _ specConfig) (n : nat) : Prop := *)
+  (*   forall l1 l2 x y, guar p x y <-> guar p (replace_lifetime x n l1) (replace_lifetime y n l2). *)
 
-  Lemma invariant_l p n (Hinv : invariant_at p n) :
-    forall l1 l2 x y, lifetime y n = Some l2 ->
-                 guar p x y <-> guar p (replace_lifetime x n l1) y.
-  Proof.
-    intros.
-    rewrite <- (replace_lifetime_same y n l2) at 2; auto.
-  Qed.
+  (* Lemma invariant_l p n (Hinv : invariant_at p n) : *)
+  (*   forall l1 l2 x y, lifetime y n = Some l2 -> *)
+  (*                guar p x y <-> guar p (replace_lifetime x n l1) y. *)
+  (* Proof. *)
+  (*   intros. *)
+  (*   rewrite <- (replace_lifetime_same y n l2) at 2; auto. *)
+  (* Qed. *)
 
-  Lemma invariant_r p n (Hinv : invariant_at p n) :
-    forall l1 l2 x y, lifetime x n = Some l1 ->
-                 guar p x y <-> guar p x (replace_lifetime y n l2).
-  Proof.
-    intros.
-    rewrite <- (replace_lifetime_same x n l1) at 2; auto.
-  Qed.
+  (* Lemma invariant_r p n (Hinv : invariant_at p n) : *)
+  (*   forall l1 l2 x y, lifetime x n = Some l1 -> *)
+  (*                guar p x y <-> guar p x (replace_lifetime y n l2). *)
+  (* Proof. *)
+  (*   intros. *)
+  (*   rewrite <- (replace_lifetime_same x n l1) at 2; auto. *)
+  (* Qed. *)
 
   (** memory helpers **)
 
@@ -364,279 +364,217 @@ Section Config.
 
   (** Lifetime permissions **)
 
-  Program Definition when (n : nat) (p : @perm _ specConfig) : perm :=
-    {|
-    pre := fun x s => (lifetime x n = Some current /\ pre p x s) \/
-                   lifetime x n = Some finished;
-    rely := fun x y => lifetime x n = None /\ lifetime y n = None \/
-                    lifetime y n = Some finished \/
-                    lifetime x n = Some current /\ lifetime y n = Some current /\ rely p x y;
-    guar := fun x y => x = y \/
-                    lifetime x n = Some current /\ lifetime y n = Some current /\ guar p x y;
-    |}.
-  Next Obligation.
-    constructor; repeat intro.
-    - destruct (lifetime x n) as [[] |]; intuition.
-    - decompose [and or] H; decompose [and or] H0; subst; auto.
-      + rewrite H1 in H3. discriminate H3.
-      + rewrite H2 in H3. discriminate H3.
-      + rewrite H1 in H2. discriminate H2.
-      + rewrite H2 in H5. discriminate H5.
-      + right; right. split; [| split]; auto. etransitivity; eauto.
-  Qed.
-  Next Obligation.
-    constructor; repeat intro; auto.
-    decompose [and or] H; decompose [and or] H0; subst; auto.
-    right. split; [| split]; auto. etransitivity; eauto.
-  Qed.
-  Next Obligation.
-    decompose [and or] H; decompose [or and] H0; subst; auto.
-    - rewrite H2 in H4. discriminate H4.
-    - rewrite H1 in H2. discriminate H2.
-    - left. split; auto. eapply pre_respects; eauto.
-    - rewrite H1 in H3. discriminate H3.
-  Qed.
+  (* Program Definition when (n : nat) (p : @perm _ specConfig) : perm := *)
+  (*   {| *)
+  (*   pre := fun x s => (lifetime x n = Some current /\ pre p x s) \/ *)
+  (*                  lifetime x n = Some finished; *)
+  (*   rely := fun x y => lifetime x n = None /\ lifetime y n = None \/ *)
+  (*                   lifetime y n = Some finished \/ *)
+  (*                   lifetime x n = Some current /\ lifetime y n = Some current /\ rely p x y; *)
+  (*   guar := fun x y => x = y \/ *)
+  (*                   lifetime x n = Some current /\ lifetime y n = Some current /\ guar p x y; *)
+  (*   |}. *)
+  (* Next Obligation. *)
+  (*   constructor; repeat intro. *)
+  (*   - destruct (lifetime x n) as [[] |]; intuition. *)
+  (*   - decompose [and or] H; decompose [and or] H0; subst; auto. *)
+  (*     + rewrite H1 in H3. discriminate H3. *)
+  (*     + rewrite H2 in H3. discriminate H3. *)
+  (*     + rewrite H1 in H2. discriminate H2. *)
+  (*     + rewrite H2 in H5. discriminate H5. *)
+  (*     + right; right. split; [| split]; auto. etransitivity; eauto. *)
+  (* Qed. *)
+  (* Next Obligation. *)
+  (*   constructor; repeat intro; auto. *)
+  (*   decompose [and or] H; decompose [and or] H0; subst; auto. *)
+  (*   right. split; [| split]; auto. etransitivity; eauto. *)
+  (* Qed. *)
+  (* Next Obligation. *)
+  (*   decompose [and or] H; decompose [or and] H0; subst; auto. *)
+  (*   - rewrite H2 in H4. discriminate H4. *)
+  (*   - rewrite H1 in H2. discriminate H2. *)
+  (*   - left. split; auto. eapply pre_respects; eauto. *)
+  (*   - rewrite H1 in H3. discriminate H3. *)
+  (* Qed. *)
 
-  Lemma when_monotone n p1 p2 : p1 <= p2 -> when n p1 <= when n p2.
-  Proof.
-    intros. destruct H. constructor; simpl; intros; decompose [and or] H; auto 7.
-  Qed.
+  (* Lemma when_monotone n p1 p2 : p1 <= p2 -> when n p1 <= when n p2. *)
+  (* Proof. *)
+  (*   intros. destruct H. constructor; simpl; intros; decompose [and or] H; auto 7. *)
+  (* Qed. *)
 
-  Instance Proper_lte_perm_when :
-    Proper (eq ==> lte_perm ==> lte_perm) when.
-  Proof.
-    repeat intro; subst. apply when_monotone; auto.
-  Qed.
+  (* Instance Proper_lte_perm_when : *)
+  (*   Proper (eq ==> lte_perm ==> lte_perm) when. *)
+  (* Proof. *)
+  (*   repeat intro; subst. apply when_monotone; auto. *)
+  (* Qed. *)
 
-  Instance Proper_eq_perm_when :
-    Proper (eq ==> eq_perm ==> eq_perm) when.
-  Proof.
-    repeat intro; subst. split; apply when_monotone; auto.
-  Qed.
+  (* Instance Proper_eq_perm_when : *)
+  (*   Proper (eq ==> eq_perm ==> eq_perm) when. *)
+  (* Proof. *)
+  (*   repeat intro; subst. split; apply when_monotone; auto. *)
+  (* Qed. *)
 
-  Lemma restrict_monotonic_at_when p n : when n p ≡ restrict_monotonic_at (when n p) n.
-  Proof.
-    split; [constructor; intros; simpl in *; auto | apply restrict_monotonic_at_lte].
-    decompose [and or] H; subst; try solve [intuition]. split; auto.
-    intro. rewrite H1, H0. reflexivity.
-  Qed.
-  Lemma when_restrict_monotonic_at p n : when n p ≡ when n (restrict_monotonic_at p n).
-  Proof.
-    split; constructor; intros; simpl in *; intuition.
-    right; intuition. intro. rewrite H, H0. reflexivity.
-  Qed.
+  (* Lemma restrict_monotonic_at_when p n : when n p ≡ restrict_monotonic_at (when n p) n. *)
+  (* Proof. *)
+  (*   split; [constructor; intros; simpl in *; auto | apply restrict_monotonic_at_lte]. *)
+  (*   decompose [and or] H; subst; try solve [intuition]. split; auto. *)
+  (*   intro. rewrite H1, H0. reflexivity. *)
+  (* Qed. *)
+  (* Lemma when_restrict_monotonic_at p n : when n p ≡ when n (restrict_monotonic_at p n). *)
+  (* Proof. *)
+  (*   split; constructor; intros; simpl in *; intuition. *)
+  (*   right; intuition. intro. rewrite H, H0. reflexivity. *)
+  (* Qed. *)
 
-  Program Definition owned (n : nat) (p : @perm _ specConfig) : (@perm _ specConfig) :=
-    {|
-    pre := fun x s => lifetime x n = Some current;
-    rely := fun x y => lifetime x n = lifetime y n /\ (lifetime x n = Some finished -> rely p x y);
-    guar := fun x y => x = y \/
-                    lifetime y n = Some finished /\ guar p (replace_lifetime x n finished) y;
-    |}.
-  Next Obligation.
-    constructor; repeat intro; auto.
-    - split; intuition.
-    - destruct H, H0.
-      split; etransitivity; eauto. apply H2. rewrite <- H. auto.
-  Qed.
-  Next Obligation.
-    constructor; repeat intro; auto.
-    decompose [and or] H; decompose [and or] H0; subst; auto.
-    right. split; auto. etransitivity; eauto.
-    rewrite <- (replace_lifetime_same y n finished); auto.
-  Qed.
+  (* Program Definition owned (n : nat) (p : @perm _ specConfig) : (@perm _ specConfig) := *)
+  (*   {| *)
+  (*   pre := fun x s => lifetime x n = Some current; *)
+  (*   rely := fun x y => lifetime x n = lifetime y n /\ (lifetime x n = Some finished -> rely p x y); *)
+  (*   guar := fun x y => x = y \/ *)
+  (*                   lifetime y n = Some finished /\ guar p (replace_lifetime x n finished) y; *)
+  (*   |}. *)
+  (* Next Obligation. *)
+  (*   constructor; repeat intro; auto. *)
+  (*   - split; intuition. *)
+  (*   - destruct H, H0. *)
+  (*     split; etransitivity; eauto. apply H2. rewrite <- H. auto. *)
+  (* Qed. *)
+  (* Next Obligation. *)
+  (*   constructor; repeat intro; auto. *)
+  (*   decompose [and or] H; decompose [and or] H0; subst; auto. *)
+  (*   right. split; auto. etransitivity; eauto. *)
+  (*   rewrite <- (replace_lifetime_same y n finished); auto. *)
+  (* Qed. *)
 
-  Lemma owned_monotone n p1 p2 : p1 <= p2 -> owned n p1 <= owned n p2.
-  Proof.
-    intros. destruct H. constructor; simpl; intros; decompose [and or] H; auto 6.
-  Qed.
+  (* Lemma owned_monotone n p1 p2 : p1 <= p2 -> owned n p1 <= owned n p2. *)
+  (* Proof. *)
+  (*   intros. destruct H. constructor; simpl; intros; decompose [and or] H; auto 6. *)
+  (* Qed. *)
 
-  Instance Proper_lte_perm_owned :
-    Proper (eq ==> lte_perm ==> lte_perm) owned.
-  Proof.
-    repeat intro; subst. apply owned_monotone; auto.
-  Qed.
+  (* Instance Proper_lte_perm_owned : *)
+  (*   Proper (eq ==> lte_perm ==> lte_perm) owned. *)
+  (* Proof. *)
+  (*   repeat intro; subst. apply owned_monotone; auto. *)
+  (* Qed. *)
 
-  Instance Proper_eq_perm_owned :
-    Proper (eq ==> eq_perm ==> eq_perm) owned.
-  Proof.
-    repeat intro; subst. split; apply owned_monotone; auto.
-  Qed.
+  (* Instance Proper_eq_perm_owned : *)
+  (*   Proper (eq ==> eq_perm ==> eq_perm) owned. *)
+  (* Proof. *)
+  (*   repeat intro; subst. split; apply owned_monotone; auto. *)
+  (* Qed. *)
 
-  Lemma restrict_monotonic_at_owned p n : owned n p ≡ restrict_monotonic_at (owned n p) n.
-  Proof.
-    split; [constructor; intros; simpl in *; auto | apply restrict_monotonic_at_lte].
-    decompose [and or] H; subst; try solve [intuition]. split; auto. clear H.
-    intro. rewrite H1. destruct (lifetime x n) as [[] |]; simpl; auto.
-  Qed.
-  Lemma owned_restrict_monotonic_at p n : owned n p ≡ owned n (restrict_monotonic_at p n).
-  Proof.
-    split; constructor; intros; simpl in *; intuition.
-    right; intuition. intro. rewrite H. rewrite lifetime_replace_lifetime. reflexivity.
-  Qed.
+  (* Lemma restrict_monotonic_at_owned p n : owned n p ≡ restrict_monotonic_at (owned n p) n. *)
+  (* Proof. *)
+  (*   split; [constructor; intros; simpl in *; auto | apply restrict_monotonic_at_lte]. *)
+  (*   decompose [and or] H; subst; try solve [intuition]. split; auto. clear H. *)
+  (*   intro. rewrite H1. destruct (lifetime x n) as [[] |]; simpl; auto. *)
+  (* Qed. *)
+  (* Lemma owned_restrict_monotonic_at p n : owned n p ≡ owned n (restrict_monotonic_at p n). *)
+  (* Proof. *)
+  (*   split; constructor; intros; simpl in *; intuition. *)
+  (*   right; intuition. intro. rewrite H. rewrite lifetime_replace_lifetime. reflexivity. *)
+  (* Qed. *)
 
-  (* trivial direction *)
-  Lemma foo' p q n :
-    owned n (restrict_monotonic_at p n * restrict_monotonic_at q n) <=
-    owned n (restrict_monotonic_at (p * q) n).
-  Proof.
-    rewrite <- owned_restrict_monotonic_at. apply owned_monotone.
-    apply sep_conj_perm_monotone; apply restrict_monotonic_at_lte.
-  Qed.
+  (* (* trivial direction *) *)
+  (* Lemma foo' p q n : *)
+  (*   owned n (restrict_monotonic_at p n * restrict_monotonic_at q n) <= *)
+  (*   owned n (restrict_monotonic_at (p * q) n). *)
+  (* Proof. *)
+  (*   rewrite <- owned_restrict_monotonic_at. apply owned_monotone. *)
+  (*   apply sep_conj_perm_monotone; apply restrict_monotonic_at_lte. *)
+  (* Qed. *)
 
-  Lemma lifetimes_sep_gen p q n :
-    p ⊥ owned n q -> when n p ⊥ owned n (p * q).
-  Proof.
-    split; intros.
-    - simpl in H0. decompose [and or] H0. subst; intuition.
-      simpl. right; left; auto.
-    - simpl in H0. decompose [and or] H0. subst; intuition.
-      simpl. split. rewrite H1, H2; auto.
-      intros. rewrite H2 in H3. discriminate H3.
-  Qed.
+  (* Lemma lifetimes_sep_gen p q n : *)
+  (*   p ⊥ owned n q -> when n p ⊥ owned n (p * q). *)
+  (* Proof. *)
+  (*   split; intros. *)
+  (*   - simpl in H0. decompose [and or] H0. subst; intuition. *)
+  (*     simpl. right; left; auto. *)
+  (*   - simpl in H0. decompose [and or] H0. subst; intuition. *)
+  (*     simpl. split. rewrite H1, H2; auto. *)
+  (*     intros. rewrite H2 in H3. discriminate H3. *)
+  (* Qed. *)
 
-  (* not actually a special case of the above *)
-  Lemma lifetimes_sep n p : when n p ⊥ owned n p.
-  Proof.
-    constructor; intros; simpl in H; auto.
-    - decompose [and or] H; subst; try reflexivity.
-      simpl. right; left; auto.
-    - decompose [and or] H; subst; try reflexivity.
-      simpl. split. rewrite H1, H0. auto. intros. rewrite H1 in H2. discriminate H2.
-  Qed.
+  (* (* not actually a special case of the above *) *)
+  (* Lemma lifetimes_sep n p : when n p ⊥ owned n p. *)
+  (* Proof. *)
+  (*   constructor; intros; simpl in H; auto. *)
+  (*   - decompose [and or] H; subst; try reflexivity. *)
+  (*     simpl. right; left; auto. *)
+  (*   - decompose [and or] H; subst; try reflexivity. *)
+  (*     simpl. split. rewrite H1, H0. auto. intros. rewrite H1 in H2. discriminate H2. *)
+  (* Qed. *)
 
-  Lemma convert p q n (Hmon : forall x y, monotonic_at p n x y) (Hmon' : forall x y, monotonic_at q n x y) :
-    when n p * owned n (p * q) <= p * owned n q.
-  Proof.
-    split; intros.
-    - simpl in *. decompose [and or] H; auto. split; auto. split; auto.
-      eapply lifetimes_sep_gen; eauto.
-    - simpl in *. decompose [and or] H; auto. destruct (lifetime x n) as [[] | ]; auto 7.
-    - simpl in H. induction H. 2: { econstructor 2; eauto. }
-      decompose [and or] H; simpl; subst; try solve [constructor; auto].
-      clear H.
-      apply Operators_Properties.clos_trans_t1n_iff.
-      apply Operators_Properties.clos_trans_t1n_iff in H2.
-      constructor 2 with (y:=replace_lifetime x n finished).
-      { right; right. split; [apply lifetime_replace_lifetime | reflexivity]. }
-      pose proof (lifetime_replace_lifetime x n finished).
-      induction H2; intros; subst; auto.
-      + constructor. destruct H1; auto. right; right. split; auto.
-        rewrite replace_lifetime_same; auto.
-      + assert (lifetime y n = Some finished).
-        { destruct H1; [apply Hmon in H1 | apply Hmon' in H1]; rewrite H in H1; simpl in H1;
-            destruct (lifetime y n) as [[] |]; inversion H1; auto. }
-        econstructor 2. 2: apply IHclos_trans_1n; auto.
-        destruct H1; auto. right; right. split; auto. rewrite replace_lifetime_same; auto.
-  Qed.
+  (* Lemma convert p q n (Hmon : forall x y, monotonic_at p n x y) (Hmon' : forall x y, monotonic_at q n x y) : *)
+  (*   when n p * owned n (p * q) <= p * owned n q. *)
+  (* Proof. *)
+  (*   split; intros. *)
+  (*   - simpl in *. decompose [and or] H; auto. split; auto. split; auto. *)
+  (*     eapply lifetimes_sep_gen; eauto. *)
+  (*   - simpl in *. decompose [and or] H; auto. destruct (lifetime x n) as [[] | ]; auto 7. *)
+  (*   - simpl in H. induction H. 2: { econstructor 2; eauto. } *)
+  (*     decompose [and or] H; simpl; subst; try solve [constructor; auto]. *)
+  (*     clear H. *)
+  (*     apply Operators_Properties.clos_trans_t1n_iff. *)
+  (*     apply Operators_Properties.clos_trans_t1n_iff in H2. *)
+  (*     constructor 2 with (y:=replace_lifetime x n finished). *)
+  (*     { right; right. split; [apply lifetime_replace_lifetime | reflexivity]. } *)
+  (*     pose proof (lifetime_replace_lifetime x n finished). *)
+  (*     induction H2; intros; subst; auto. *)
+  (*     + constructor. destruct H1; auto. right; right. split; auto. *)
+  (*       rewrite replace_lifetime_same; auto. *)
+  (*     + assert (lifetime y n = Some finished). *)
+  (*       { destruct H1; [apply Hmon in H1 | apply Hmon' in H1]; rewrite H in H1; simpl in H1; *)
+  (*           destruct (lifetime y n) as [[] |]; inversion H1; auto. } *)
+  (*       econstructor 2. 2: apply IHclos_trans_1n; auto. *)
+  (*       destruct H1; auto. right; right. split; auto. rewrite replace_lifetime_same; auto. *)
+  (* Qed. *)
 
-  (* special case of convert *)
-  Lemma convert_bottom p n (Hmon : forall x y, monotonic_at p n x y) :
-    when n p * owned n p <= p * owned n bottom_perm.
-  Proof.
-    rewrite <- (sep_conj_perm_bottom p) at 2. apply convert; auto.
-    repeat intro. simpl in H. subst. reflexivity.
-  Qed.
+  (* (* special case of convert *) *)
+  (* Lemma convert_bottom p n (Hmon : forall x y, monotonic_at p n x y) : *)
+  (*   when n p * owned n p <= p * owned n bottom_perm. *)
+  (* Proof. *)
+  (*   rewrite <- (sep_conj_perm_bottom p) at 2. apply convert; auto. *)
+  (*   repeat intro. simpl in H. subst. reflexivity. *)
+  (* Qed. *)
 
   (** memory permissions **)
-
-  (* Program Definition read_p (ptr : addr) : perm := *)
-  (*   {| *)
-  (*   (* ptr points to valid memory *) *)
-  (*   pre x := exists v, read x ptr = Some v; *)
-  (*   (* only checks if the memory ptr points to in the 2 configs are equal *) *)
-  (*   rely x y := alloc_invariant x y ptr; *)
-  (*   (* read x ptr = None <-> read y ptr = None; *) *)
-  (*   (* only the pointer we have write permission to may change *) *)
-  (*   guar x y := x = y; *)
-  (*   |}. *)
-  (* Next Obligation. *)
-  (*   constructor; unfold alloc_invariant; unfold allocated; repeat intro; auto. *)
-  (*   destruct (m x (fst ptr)), (m y (fst ptr)), (m z (fst ptr)); intuition. *)
-  (*   - destruct l0, l1, l2. *)
-  (*     destruct (bytes (snd ptr)), (bytes0 (snd ptr)), (bytes1 (snd ptr)); subst; *)
-  (*       etransitivity; eauto. *)
-  (*   - destruct l0, l1. *)
-  (*     destruct (bytes (snd ptr)), (bytes0 (snd ptr)); subst; *)
-  (*       etransitivity; eauto. *)
-  (*   - destruct l0, l1. *)
-  (*     destruct (bytes (snd ptr)), (bytes0 (snd ptr)); subst; *)
-  (*       etransitivity; eauto. *)
-  (*   - destruct l0, l1. *)
-  (*     destruct (bytes (snd ptr)), (bytes0 (snd ptr)); subst; *)
-  (*       etransitivity; eauto. *)
-  (* Qed. *)
-  (* Next Obligation. *)
-  (*   destruct (read y ptr) eqn:?. *)
-  (*   eexists; eauto. *)
-  (*   assert ((None : option SByte) = None) by reflexivity. *)
-  (*   eapply alloc_invariant_read in Heqo; eauto. rewrite H1 in Heqo. inversion Heqo. *)
-  (* Qed. *)
-  (* Next Obligation. *)
-  (*   constructor; repeat intro; auto. etransitivity; eauto. *)
-  (* Qed. *)
-
-  (* (* TODO factor out common pre and rely *) *)
-  (* Program Definition write_p (ptr : addr) : perm := *)
-  (*   {| *)
-  (*   (* ptr points to valid memory *) *)
-  (*   pre x := exists v, read x ptr = Some v; *)
-  (*   (* only checks if the memory ptr points to in the 2 configs are equal *) *)
-  (*   rely x y := read x ptr = read y ptr; *)
-  (*   (* only the pointer we have write permission to may change *) *)
-  (*   (* TODO: cannot dealloc or alloc here... *) *)
-  (*   guar x y := (forall ptr', ptr <> ptr' -> read x ptr' = read y ptr') /\ *)
-  (*              alloc_invariant x y ptr; *)
-  (*   |}. *)
-  (* Next Obligation. *)
-  (*   constructor; repeat intro; auto. etransitivity; eauto. *)
-  (* Qed. *)
-  (* Next Obligation. *)
-  (*   eexists; eauto. *)
-  (* Qed. *)
-  (* Next Obligation. *)
-  (*   constructor; split; repeat intro; try solve [intuition]. *)
-  (*   - reflexivity. *)
-  (*   - destruct H, H0. etransitivity. apply H; auto. auto. *)
-  (*   - destruct H, H0. etransitivity. apply H1. auto. *)
-  (* Qed. *)
 
   Program Definition read_perm (ptr : addr) (v : SByte) : (@perm _ specConfig) :=
     {|
     (* ptr points to valid memory *)
-    pre x s := read x ptr = Some v;
+    pre '(x, _) := read x ptr = Some v;
     (* only checks if the memory ptr points to in the 2 configs are equal *)
-    rely x y := read x ptr = read y ptr;
+    rely '(x, _) '(y, _) := read x ptr = read y ptr;
     (* no guarates allowed *)
-    guar x y := x = y;
+    guar '(x, _) '(y, _) := x = y;
     |}.
   Next Obligation.
-    constructor; repeat intro; auto. etransitivity; eauto.
+    constructor; [intros [] | intros [] [] []]; auto; etransitivity; eauto.
   Qed.
   Next Obligation.
-    constructor; repeat intro; subst; auto.
+    constructor; [intros [] | intros [] [] [] ? ?]; subst; auto.
   Qed.
 
   Program Definition write_perm (ptr : addr) (v : SByte) : (@perm _ specConfig) :=
     {|
     (* ptr points to valid memory *)
-    pre x s := read x ptr = Some v;
+    pre '(x, _) := read x ptr = Some v;
     (* only checks if the memory ptr points to in the 2 configs are equal *)
-    rely x y := read x ptr = read y ptr;
+    rely '(x, _) '(y, _) := read x ptr = read y ptr;
     (* only the pointer we have write permission to may change *)
-    guar x y := (forall ptr', ptr <> ptr' -> read x ptr' = read y ptr') /\
-                alloc_invariant x y ptr /\
-                l x = l y
+    guar '(x, _) '(y, _) := (forall ptr', ptr <> ptr' -> read x ptr' = read y ptr') /\
+                            alloc_invariant x y ptr /\
+                            l x = l y
     |}.
   Next Obligation.
-    constructor; repeat intro; auto. etransitivity; eauto.
+    constructor; [intros [] | intros [] [] []]; auto; etransitivity; eauto.
   Qed.
   Next Obligation.
-    constructor; split; repeat intro; try solve [intuition].
-    - split; [| split]; reflexivity.
-    - destruct H, H0. etransitivity. apply H; auto. auto.
-    - destruct H as (? & ? & ?), H0 as (? & ? & ?).
-      split; etransitivity; eauto.
+    constructor.
+    - intros []; split; [| split]; intros; reflexivity.
+    - intros [] [] [] (? & ? & ?) (? & ? & ?); split; [| split]; intros; try congruence.
+      etransitivity. apply H; auto. apply H2; auto.
   Qed.
 
   Definition read_Perms (ptr : addr) (P : SByte -> Perms) : Perms :=
@@ -647,45 +585,45 @@ Section Config.
 
   Lemma read_lte_write : forall ptr v, read_perm ptr v <= write_perm ptr v.
   Proof.
-    constructor; simpl; repeat intro; subst; auto.
+    constructor; simpl; intros [] []; subst; auto. intros; subst.
     split; [| split; [| split]]; intros; reflexivity.
   Qed.
 
-  Lemma read_write_separate_neq_ptr : forall ptr ptr' v v',
-      read_perm ptr v ⊥ write_perm ptr' v' <-> ptr <> ptr'.
-  Proof.
-    split; repeat intro.
-    - destruct H as [? _]. simpl in *. subst.
-      specialize (sep_l (config_mem ptr' (Byte 0)) (config_mem ptr' (Byte 1))).
-      do 2 rewrite read_config_mem in sep_l.
-      assert (Some (Byte 0) = Some (Byte 1) -> False) by inversion 1.
-      apply H. clear H. apply sep_l. split; [| split; [| split]]; auto.
-      + intros. unfold read, config_mem. simpl.
-        destruct ptr', ptr'0. destruct (addr_neq_cases _ _ _ _ H); simpl in *.
-        * rewrite (Bool.reflect_iff _ _ (Nat.eqb_spec _ _)) in H0.
-          apply Bool.not_true_is_false in H0. rewrite Nat.eqb_sym in H0.
-          rewrite H0. auto.
-        * destruct (n1 =? n); auto. destruct (n2 <? n0 + 1); auto.
-          rewrite (Bool.reflect_iff _ _ (Nat.eqb_spec _ _)) in H0.
-          apply Bool.not_true_is_false in H0. rewrite Nat.eqb_sym in H0.
-          rewrite H0. auto.
-      + unfold alloc_invariant, allocated, config_mem. simpl.
-        repeat rewrite Nat.eqb_refl. auto.
-    - constructor; intros; simpl in *; subst; auto.
-      destruct H0. auto.
-  Qed.
+  (* Lemma read_write_separate_neq_ptr : forall ptr ptr' v v', *)
+  (*     read_perm ptr v ⊥ write_perm ptr' v' <-> ptr <> ptr'. *)
+  (* Proof. *)
+  (*   split; repeat intro. *)
+  (*   - destruct H as [? _]. simpl in *. subst. *)
+  (*     specialize (sep_l (config_mem ptr' (Byte 0)) (config_mem ptr' (Byte 1))). *)
+  (*     do 2 rewrite read_config_mem in sep_l. *)
+  (*     assert (Some (Byte 0) = Some (Byte 1) -> False) by inversion 1. *)
+  (*     apply H. clear H. apply sep_l. split; [| split; [| split]]; auto. *)
+  (*     + intros. unfold read, config_mem. simpl. *)
+  (*       destruct ptr', ptr'0. destruct (addr_neq_cases _ _ _ _ H); simpl in *. *)
+  (*       * rewrite (Bool.reflect_iff _ _ (Nat.eqb_spec _ _)) in H0. *)
+  (*         apply Bool.not_true_is_false in H0. rewrite Nat.eqb_sym in H0. *)
+  (*         rewrite H0. auto. *)
+  (*       * destruct (n1 =? n); auto. destruct (n2 <? n0 + 1); auto. *)
+  (*         rewrite (Bool.reflect_iff _ _ (Nat.eqb_spec _ _)) in H0. *)
+  (*         apply Bool.not_true_is_false in H0. rewrite Nat.eqb_sym in H0. *)
+  (*         rewrite H0. auto. *)
+  (*     + unfold alloc_invariant, allocated, config_mem. simpl. *)
+  (*       repeat rewrite Nat.eqb_refl. auto. *)
+  (*   - constructor; intros; simpl in *; subst; auto. *)
+  (*     destruct H0. auto. *)
+  (* Qed. *)
 
-  Lemma write_write_separate_neq_ptr : forall ptr ptr' v v',
-      write_perm ptr v ⊥ write_perm ptr' v' <-> ptr <> ptr'.
-  Proof.
-    split; intros.
-    - symmetry in H. eapply separate_antimonotone in H. symmetry in H.
-      eapply read_write_separate_neq_ptr. apply H. apply read_lte_write.
-    - constructor; intros; simpl in *; destruct H0; auto.
-  Qed.
+  (* Lemma write_write_separate_neq_ptr : forall ptr ptr' v v', *)
+  (*     write_perm ptr v ⊥ write_perm ptr' v' <-> ptr <> ptr'. *)
+  (* Proof. *)
+  (*   split; intros. *)
+  (*   - symmetry in H. eapply separate_antimonotone in H. symmetry in H. *)
+  (*     eapply read_write_separate_neq_ptr. apply H. apply read_lte_write. *)
+  (*   - constructor; intros; simpl in *; destruct H0; auto. *)
+  (* Qed. *)
 
-  Lemma read_separate : forall ptr ptr' v v', read_perm ptr v ⊥ read_perm ptr' v'.
-  Proof.
-    constructor; intros; simpl in *; subst; reflexivity.
-  Qed.
+  (* Lemma read_separate : forall ptr ptr' v v', read_perm ptr v ⊥ read_perm ptr' v'. *)
+  (* Proof. *)
+  (*   constructor; intros; simpl in *; subst; reflexivity. *)
+  (* Qed. *)
 End Config.
